src/asn1/ASN1.Low.Value.fst
@@ -6,4 +6,5 @@ include ASN1.Low.Value.INTEGER
 include ASN1.Low.Value.OCTET_STRING
 include ASN1.Low.Value.BIT_STRING
 include ASN1.Low.Value.OID
+include ASN1.Low.Value.Envelop
 include ASN1.Low.Value.SEQUENCE
