src/asn1/ASN1.Spec.Value.Envelop.fst
@@ -1,0 +1,278 @@
+module ASN1.Spec.Value.Envelop
+
+open ASN1.Base
+open ASN1.Spec.Tag
+open ASN1.Spec.Length
+open LowParse.Bytes
+open LowParse.Spec.FLData
+
+open FStar.Integers
+
+(* NOTE: Read after `ASN1.Spec.Tag`, `ASN1.Spec.Length`, `ASN1.Spec.Value.*` *)
+
+(* NOTE: Use `parse_fldata_strong` to construct fixed-length parsers (with the strong prefix proeprty),
+         where these fixed-length is runtimely parsed.
+ *)
+
+/// Tagging function
+///
+noextract
+let parser_tag_of_asn1_envelop_tag_with
+  (#k: parser_kind)
+  (#t: Type0)
+  (#p: parser k t)
+  (a: asn1_type)
+  (s: serializer p)
+  (data: t { asn1_value_length_inbound_of_type a (Seq.length (serialize s data)) } )
+: GTot (the_asn1_type a & asn1_value_int32_of_type a)
+= (a, u (Seq.length (serialize s data)))
+
+noextract
+let synth_asn1_envelop_tag_with
+  (#k: parser_kind)
+  (#t: Type0)
+  (#p: parser k t)
+  (a: asn1_type)
+  (s: serializer p)
+  (tag: (the_asn1_type a & asn1_value_int32_of_type a))
+  (y: parse_fldata_strong_t s (v (snd tag)))
+: GTot (refine_with_tag (parser_tag_of_asn1_envelop_tag_with a s) tag)
+= y <: refine_with_tag (parser_tag_of_asn1_envelop_tag_with a s) tag
+
+noextract
+let synth_asn1_envelop_tag_with_inverse
+  (#k: parser_kind)
+  (#t: Type0)
+  (#p: parser k t)
+  (a: asn1_type)
+  (s: serializer p)
+  (tag: (the_asn1_type a & asn1_value_int32_of_type a))
+  (data: refine_with_tag (parser_tag_of_asn1_envelop_tag_with a s) tag)
+: GTot (y: parse_fldata_strong_t s (v (snd tag)){ data == synth_asn1_envelop_tag_with a s tag y })
+= data <: refine_with_tag (parser_tag_of_asn1_envelop_tag_with a s) tag
+
+/// ASN.1 a value parser/serializer
+///
+noextract
+let parse_asn1_envelop_tag_with
+  (#k: parser_kind)
+  (#t: Type0)
+  (#p: parser k t)
+  (a: asn1_type)
+  (s: serializer p)
+  (tag: the_asn1_type a & asn1_value_int32_of_type a)
+: parser (parse_fldata_kind (v (snd tag)) k) (refine_with_tag (parser_tag_of_asn1_envelop_tag_with a s) tag)
+= serializer_correct_implies_complete p s;
+  parse_fldata_strong s (v (snd tag))
+  `parse_synth`
+  synth_asn1_envelop_tag_with a s tag
+
+noextract
+let lemma_parse_asn1_envelop_tag_with_unfold
+  (#k: parser_kind)
+  (#t: Type0)
+  (#p: parser k t)
+  (a: asn1_type)
+  (s: serializer p)
+  (tag: the_asn1_type a & asn1_value_int32_of_type a)
+  (input: bytes)
+: Lemma (
+  parse (parse_asn1_envelop_tag_with a s tag) input ==
+ (match parse (parse_fldata_strong s (v (snd tag))) input with
+  | None -> None
+  | Some (value, consumed) -> Some (synth_asn1_envelop_tag_with a s tag value, consumed)))
+= parse_synth_eq
+  (* p1 *) (parse_fldata_strong s (v (snd tag)))
+  (* f2 *) (synth_asn1_envelop_tag_with a s tag)
+  (* in *) (input)
+
+noextract
+let parse_asn1_envelop_tag_with_weak
+  (#k: parser_kind)
+  (#t: Type0)
+  (#p: parser k t)
+  (a: asn1_type)
+  (s: serializer p)
+  (tag: the_asn1_type a & asn1_value_int32_of_type a)
+: parser (weak_kind_of_type a) (refine_with_tag (parser_tag_of_asn1_envelop_tag_with a s) tag)
+= weak_kind_of_type a
+  `weaken`
+  parse_asn1_envelop_tag_with a s tag
+
+noextract
+let serialize_asn1_envelop_tag_with
+  (#k: parser_kind)
+  (#t: Type0)
+  (#p: parser k t)
+  (a: asn1_type)
+  (s: serializer p)
+  (tag: the_asn1_type a & asn1_value_int32_of_type a)
+: serializer (parse_asn1_envelop_tag_with a s tag)
+= serializer_correct_implies_complete p s;
+  serialize_synth
+  (* p1 *) (parse_fldata_strong s (v (snd tag)))
+  (* f2 *) (synth_asn1_envelop_tag_with a s tag)
+  (* s1 *) (serialize_fldata_strong s (v (snd tag)))
+  (* g1 *) (synth_asn1_envelop_tag_with_inverse a s tag)
+  (* prf*) ()
+
+noextract
+let lemma_serialize_asn1_envelop_tag_with_unfold
+  (#k: parser_kind)
+  (#t: Type0)
+  (#p: parser k t)
+  (a: asn1_type)
+  (s: serializer p)
+  (tag: the_asn1_type a & asn1_value_int32_of_type a)
+  (value: refine_with_tag (parser_tag_of_asn1_envelop_tag_with a s) tag)
+: Lemma (
+  serialize
+    (serialize_fldata_strong s (v (snd tag)))
+    (synth_asn1_envelop_tag_with_inverse a s tag value)
+  == serialize (serialize_asn1_envelop_tag_with a s tag) value
+)
+= serializer_correct_implies_complete p s;
+  serialize_synth_eq
+  (* p1 *) (parse_fldata_strong s (v (snd tag)))
+  (* f2 *) (synth_asn1_envelop_tag_with a s tag)
+  (* s1 *) (serialize_fldata_strong s (v (snd tag)))
+  (* g1 *) (synth_asn1_envelop_tag_with_inverse a s tag)
+  (* prf*) ()
+  (* val*) (value)
+
+noextract
+let serialize_asn1_envelop_tag_with_weak
+  (#k: parser_kind)
+  (#t: Type0)
+  (#p: parser k t)
+  (a: asn1_type)
+  (s: serializer p)
+  (tag: the_asn1_type a & asn1_value_int32_of_type a)
+: serializer (parse_asn1_envelop_tag_with_weak a s tag)
+= weak_kind_of_type a
+  `serialize_weaken`
+  serialize_asn1_envelop_tag_with a s tag
+
+/// Specialized TLV parser/serializer
+///
+///
+
+let parse_asn1_envelop_tag_with_TLV_kind
+  (a: asn1_type)
+: parser_kind
+= parse_asn1_tag_kind
+  `and_then_kind`
+  parse_asn1_length_kind_of_type a
+  `and_then_kind`
+  weak_kind_of_type a
+
+noextract
+let parse_asn1_envelop_tag_with_TLV
+  (#k: parser_kind)
+  (#t: Type0)
+  (#p: parser k t)
+  (a: asn1_type)
+  (s: serializer p)
+: parser (parse_asn1_envelop_tag_with_TLV_kind a) (x: t{ asn1_value_length_inbound_of_type a (Seq.length (serialize s x)) })
+= parse_tagged_union
+  (* pt *) (parse_asn1_tag_of_type a
+            `nondep_then`
+            parse_asn1_length_of_type a)
+  (* tg *) (parser_tag_of_asn1_envelop_tag_with a s)
+  (* p  *) (parse_asn1_envelop_tag_with_weak a s)
+
+noextract
+let serialize_asn1_envelop_tag_with_TLV
+  (#k: parser_kind)
+  (#t: Type0)
+  (#p: parser k t)
+  (a: asn1_type)
+  (s: serializer p)
+: Tot (serializer (parse_asn1_envelop_tag_with_TLV a s))
+= serialize_tagged_union
+  (* st *) (serialize_asn1_tag_of_type a
+            `serialize_nondep_then`
+            serialize_asn1_length_of_type a)
+  (* tg *) (parser_tag_of_asn1_envelop_tag_with a s)
+  (* s  *) (serialize_asn1_envelop_tag_with_weak a s)
+
+#push-options "--query_stats --z3rlimit 32"
+let lemma_serialize_asn1_envelop_tag_with_TLV_unfold
+  (#k: parser_kind)
+  (#t: Type0)
+  (#p: parser k t)
+  (a: asn1_type)
+  (s: serializer p)
+  (value: t{ asn1_value_length_inbound_of_type a (Seq.length (serialize s value)) })
+: Lemma (
+  serialize (serialize_asn1_envelop_tag_with_TLV a s) value ==
+  serialize (serialize_asn1_tag_of_type a) a
+  `Seq.append`
+  serialize (serialize_asn1_length_of_type a) (u (Seq.length (serialize (serialize_asn1_envelop_tag_with a s (parser_tag_of_asn1_envelop_tag_with a s value)) value)))
+  `Seq.append`
+  serialize (serialize_asn1_envelop_tag_with a s (parser_tag_of_asn1_envelop_tag_with a s value)) value
+  // /\
+  // serialize (serialize_asn1_envelop_tag_with_tlv a s) value ==
+  // serialize (serialize_asn1_tag_of_type sequence) sequence
+  // `seq.append`
+  // serialize (serialize_asn1_length_of_type sequence) (u (seq.length (serialize s value)))
+  // `seq.append`
+  // serialize s value
+)
+= //lemma_serialize_asn1_envelop_tag_with_unfold s (parser_tag_of_asn1_envelop_tag_with s value) value;
+  serialize_nondep_then_eq
+  (* s1 *) (serialize_asn1_tag_of_type a)
+  (* s2 *) (serialize_asn1_length_of_type a)
+  (* val*) (parser_tag_of_asn1_envelop_tag_with a s value);
+  serialize_tagged_union_eq
+  (* st *) (serialize_asn1_tag_of_type a
+            `serialize_nondep_then`
+            serialize_asn1_length_of_type a)
+  (* tg *) (parser_tag_of_asn1_envelop_tag_with a s)
+  (* s  *) (serialize_asn1_envelop_tag_with_weak a s)
+  (* val*) (value)
+
+noextract
+let lemma_serialize_asn1_envelop_tag_with_TLV_size
+  (#k: parser_kind)
+  (#t: Type0)
+  (#p: parser k t)
+  (a: asn1_type)
+  (s: serializer p)
+  (value: t{ asn1_value_length_inbound_of_type a (Seq.length (serialize s value)) })
+: Lemma (
+  let length: asn1_value_length_of_type a = Seq.length (serialize s value) in
+  let len: asn1_value_int32_of_type a = u length in
+  Seq.length (serialize (serialize_asn1_envelop_tag_with_TLV a s) value) ==
+  1 + length_of_asn1_length len + length)
+= let length: asn1_value_length_of_type a = Seq.length (serialize s value) in
+  let len: asn1_value_int32_of_type a = u length in
+  lemma_serialize_asn1_envelop_tag_with_TLV_unfold a s value;
+  lemma_serialize_asn1_tag_of_type_size a a;
+  lemma_serialize_asn1_length_size len;
+  serialize_asn1_length_of_type_eq a len
+
+noextract
+let length_of_envelop_tag_with_TLV
+  (#k: parser_kind)
+  (#t: Type0)
+  (#p: parser k t)
+  (a: asn1_type)
+  (s: serializer p)
+  (value: t{ asn1_value_length_inbound_of_type a (Seq.length (serialize s value)) })
+: GTot (l: asn1_TLV_length_of_type a { l == Seq.length (serialize (serialize_asn1_envelop_tag_with_TLV a s) value) })
+= let length = Seq.length (serialize s value) in
+  let len: asn1_int32 = u length in
+  lemma_serialize_asn1_envelop_tag_with_TLV_unfold a s value;
+  lemma_serialize_asn1_envelop_tag_with_TLV_size a s value;
+  1 + length_of_asn1_length len + length
+#pop-options
+
+unfold
+let inbound_envelop_tag_with_value_of
+  (#k: parser_kind)
+  (#t: Type0)
+  (#p: parser k t)
+  (a: asn1_type)
+  (s: serializer p)
+= x: t{ asn1_value_length_inbound_of_type a (Seq.length (serialize s x)) }
