src/asn1/RIoT.Test.fst
@@ -1,0 +1,153 @@
+module RIoT.Test
+
+open LowParse.Low.Base
+open LowParse.Low.Combinators
+
+open ASN1.Spec
+open ASN1.Low
+
+module U8 = FStar.UInt8
+module U32 = FStar.UInt32
+module HS = FStar.HyperStack
+module HST = FStar.HyperStack.ST
+module MB = LowStar.Monotonic.Buffer
+module B = LowStar.Buffer
+module Cast = FStar.Int.Cast
+module C = C
+module B32 = FStar.Bytes
+
+open X509.Crypto
+open X509.RIoT
+
+open Lib.IntTypes
+friend Lib.IntTypes
+
+module I = FStar.Integers
+
+module S = Spec.Hash.Definitions
+module H = Hacl.Hash.Definitions
+// module Ed25519 = Hacl.Ed25519
+// module Curve25519 = Hacl.Curve25519_51
+module ECDSA = Hacl.Impl.ECDSA
+module P256 = Hacl.Impl.P256
+module HKDF = Hacl.HKDF
+
+let key_t = B.lbuffer uint8 32
+let sig_t = B.lbuffer uint8 64
+
+(* ZT: Some tests to indicate if the proof performance has been
+       affected by some definitions from ASN1.* or Hacl.* *)
+let _ = assert (length_of_oid OID_EC_GRP_SECP256R1 == 6)
+let _ = assert (length_of_asn1_primitive_TLV (Mkbit_string_t 33ul 0ul (magic())) == 35)
+
+
+#restart-solver
+#push-options "--query_stats --z3rlimit 32"
+let x509GetAliasCertTBS
+  (tbs_len: size_t)
+  (tbs: B.lbuffer uint8 (v tbs_len))
+  (tbs_pos: size_t)
+  (version: datatype_of_asn1_type INTEGER)
+  (aliasKeyPub: key_t)
+  (deviceKeyPub: key_t)
+  (fwid_len: asn1_value_int32_of_type OCTET_STRING)
+  (fwid: B.lbuffer uint8 (v fwid_len))
+: HST.StackInline (size_t)
+  (requires fun h ->
+    B.all_live h [B.buf tbs;
+                  B.buf aliasKeyPub;
+                  B.buf deviceKeyPub;
+                  B.buf fwid] /\
+    B.all_disjoint [B.loc_buffer tbs;
+                    B.loc_buffer aliasKeyPub;
+                    B.loc_buffer deviceKeyPub;
+                    B.loc_buffer fwid] /\
+    0 <= v tbs_pos /\ v tbs_pos <= v tbs_len /\
+    v fwid_len < asn1_length_max - 86 /\
+   (let compositeDeviceID = constructCompositeDeviceID
+                            (* version  *) version
+                            (* devKeyPub*) (B32.hide (B.as_seq h deviceKeyPub))
+                            (* fwid_len *) fwid_len
+                            (* fwid     *) (B32.hide (B.as_seq h fwid)) in
+    let offset = Seq.length (serialize serialize_compositeDeviceID_sequence_TLV compositeDeviceID) in
+    offset <= v tbs_pos))
+  (ensures fun h0 offset h1 ->
+    B.modifies (B.loc_buffer_from_to tbs (tbs_pos -! offset) tbs_pos) h0 h1 (* TODO: refine locs *))
+= let compositeDeviceID = constructCompositeDeviceID
+                          (* version  *) version
+                          (* devKeyPub*) (B32.of_buffer 32ul deviceKeyPub)
+                          (* fwid_len *) fwid_len
+                          (* fwid     *) (B32.of_buffer fwid_len fwid) in
+  let offset = serialize32_compositeDeviceID_TLV_sequence_backwards
+               (* val *) compositeDeviceID
+               (* buf *) tbs
+               (* pos *) tbs_pos in
+  let aliasPubKeyInfo = x509GetAliasKeyInfo (B32.of_buffer 32ul aliasKeyPub) in
+offset
+#pop-options
+
+let () = ()
+
+
+#restart-solver
+#push-options "--query_stats --z3rlimit 64"
+let main ()
+: HST.St C.exit_code
+= HST.push_frame ();
+
+  let private_key = B.alloca 0x00uy 32ul in
+  let public_key = Ed25519.secret_to_public private_key in
+
+  (* Create TBS region for Alias Key *)
+  let buf_len = 500ul in
+  let buf = B.alloca 0x00uy buf_len in
+
+  // let algo_oid: b: B.buffer uint8 {B.length b == 2} = B.alloca 0x05uy 2ul in
+  // let algo_param: b: B.buffer uint8 {B.length b == 5} = B.alloca 0x01uy 5ul in
+  // let algo_id: algorithmIdentifier_t = {
+  //   algorithm_oid = (|2ul, B32.of_buffer 2ul algo_oid|);
+  //   parameters    = (|5ul, B32.of_buffer 5ul algo_param|)
+  // } in
+
+  //   (* NOTE: We need to prove this whole constructed SEQUENCE value has a valid length frist. *)
+  // (* Prf *) serialize_algorithmIdentifier_value_unfold algo_id;
+  // (* Prf *) lemma_serialize_asn1_octet_string_TLV_size algo_id.algorithm_oid;
+  // (* Prf *) lemma_serialize_asn1_octet_string_TLV_size algo_id.parameters;
+
+  // (* NOTE: Then reveal the whole constructed SEQUENCE TLV's length. *)
+  // // (* Prf *) serialize_algorithmIdentifier_sequence_unfold algo_id;
+  // (* Prf *) serialize_algorithmIdentifier_sequence_TLV_size algo_id;
+
+  // let pubkey: b: B.buffer uint8 {B.length b == 3} = B.alloca 0b100uy 3ul in
+  // let subjectPublicKeyInfo: subjectPublicKeyInfo_t = {
+  //   algorithm = algo_id;
+  //                      (* FIXME: conflicting with `LowParse.Slice.slice` *)
+  //   subjectPublicKey = Mkbit_string_t 4ul 2ul (B32.of_buffer 3ul pubkey)
+  // } in
+
+  // (* NOTE: Prove subjectPublicKeyInfo is inbound. *)
+  // (* Prf *) serialize_subjectPublicKeyInfo_value_unfold subjectPublicKeyInfo;
+  // (* Prf *) lemma_serialize_asn1_bit_string_TLV_size subjectPublicKeyInfo.subjectPublicKey;
+
+  // (* NOTE: Reveal subjectPublicKeyInfo's TLV's length. *)
+  // (* Prf *) serialize_subjectPublicKeyInfo_sequence_TLV_size subjectPublicKeyInfo;
+
+  // let offset = serialize32_subjectPublicKeyInfo_sequence_TLV_backwards
+  //              (* val *) subjectPublicKeyInfo
+  //              (* buf *) buf
+  //              (* pos *) buf_len in
+
+  let offset = 50ul in
+
+  let aliasSig = B.alloca 0x00uy 64ul in
+  let aliasTBS = B.sub buf (buf_len -! offset) offset in
+
+  Ed25519.sign
+    (* sig *) aliasSig
+    (* priv*) private_key
+    (* len *) offset
+    (* msg *) aliasTBS;
+
+  HST.pop_frame ();
+  C.EXIT_SUCCESS
+#pop-options
