src/asn1/RIot.Ext.CompositeDeviceID.fst
@@ -1,0 +1,167 @@
+module RIoT.Ext.CompositeDeviceID
+
+open LowParse.Low.Base
+open LowParse.Low.Combinators
+
+open ASN1.Spec
+open ASN1.Low
+
+open RIoT.Ext
+
+
+//////////////////////////////////////////////////////////
+noeq
+type compositeDeviceID_t = {
+  version: datatype_of_asn1_type INTEGER;
+  deviceID: subjectPublicKeyInfo_t_inbound;
+  fwid2: fwid_t_inbound
+}
+
+let compositeDeviceID_t' = ((datatype_of_asn1_type INTEGER * subjectPublicKeyInfo_t_inbound) * fwid_t_inbound)
+
+(* Serialier spec *)
+let synth_compositeDeviceID_t
+  (x': compositeDeviceID_t')
+: GTot (compositeDeviceID_t)
+= { version  = fst (fst x');
+    deviceID = snd (fst x');
+    fwid2     = snd x' }
+
+let synth_compositeDeviceID_t'
+  (x: compositeDeviceID_t)
+: Tot (x': compositeDeviceID_t' { x == synth_compositeDeviceID_t x' })
+= let a: (datatype_of_asn1_type INTEGER * subjectPublicKeyInfo_t_inbound) = (x.version, x.deviceID) in
+  (a, x.fwid2)
+
+let parse_compositeDeviceID_value
+: parser _ compositeDeviceID_t
+= parse_asn1_TLV_of_type INTEGER
+  `nondep_then`
+  parse_subjectPublicKeyInfo_sequence_TLV
+  `nondep_then`
+  parse_fwid_sequence_TLV
+  `parse_synth`
+  synth_compositeDeviceID_t
+
+let serialize_compositeDeviceID_value
+: serializer parse_compositeDeviceID_value
+= serialize_synth
+  (* p1 *) (parse_asn1_TLV_of_type INTEGER
+            `nondep_then`
+            parse_subjectPublicKeyInfo_sequence_TLV
+            `nondep_then`
+            parse_fwid_sequence_TLV)
+  (* f2 *) (synth_compositeDeviceID_t)
+  (* s1 *) (serialize_asn1_TLV_of_type INTEGER
+            `serialize_nondep_then`
+            serialize_subjectPublicKeyInfo_sequence_TLV
+            `serialize_nondep_then`
+            serialize_fwid_sequence_TLV)
+  (* g1 *) (synth_compositeDeviceID_t')
+  (* prf*) ()
+
+let serialize_compositeDeviceID_value_unfold
+  (x: compositeDeviceID_t)
+: Lemma (
+  serialize serialize_compositeDeviceID_value x ==
+  serialize (serialize_asn1_TLV_of_type INTEGER) x.version
+  `Seq.append`
+  serialize serialize_subjectPublicKeyInfo_sequence_TLV x.deviceID
+  `Seq.append`
+  serialize serialize_fwid_sequence_TLV x.fwid2
+)
+= serialize_nondep_then_eq
+  (* s1 *) (serialize_asn1_TLV_of_type INTEGER)
+  (* s2 *) (serialize_subjectPublicKeyInfo_sequence_TLV)
+  (* in *) (fst (synth_compositeDeviceID_t' x));
+  serialize_nondep_then_eq
+  (* s1 *) (serialize_asn1_TLV_of_type INTEGER
+            `serialize_nondep_then`
+            serialize_subjectPublicKeyInfo_sequence_TLV)
+  (* s2 *) (serialize_fwid_sequence_TLV)
+  (* in *) (synth_compositeDeviceID_t' x);
+  serialize_synth_eq
+  (* p1 *) (parse_asn1_TLV_of_type INTEGER
+            `nondep_then`
+            parse_subjectPublicKeyInfo_sequence_TLV
+            `nondep_then`
+            parse_fwid_sequence_TLV)
+  (* f2 *) (synth_compositeDeviceID_t)
+  (* s1 *) (serialize_asn1_TLV_of_type INTEGER
+            `serialize_nondep_then`
+            serialize_subjectPublicKeyInfo_sequence_TLV
+            `serialize_nondep_then`
+            serialize_fwid_sequence_TLV)
+  (* g1 *) (synth_compositeDeviceID_t')
+  (* prf*) ()
+  (* in *) x
+open FStar.Integers
+
+let serialize_compositeDeviceID_value_size
+  (x: compositeDeviceID_t)
+: Lemma (
+  Seq.length (serialize serialize_compositeDeviceID_value x) ==
+  length_of_asn1_primitive_TLV x.version +
+  v (len_of_subjectPublicKeyInfo_TLV_inbound x.deviceID) +
+  v (len_of_fwid_TLV_inbound x.fwid2))
+= serialize_compositeDeviceID_value_unfold x;
+  lemma_serialize_asn1_integer_TLV_size x.version;
+  serialize_subjectPublicKeyInfo_sequence_TLV_size x.deviceID;
+  serialize_fwid_sequence_TLV_size x.fwid2
+
+(* inbound sub type*)
+let compositeDeviceID_t_inbound
+= inbound_sequence_value_of serialize_compositeDeviceID_value
+
+(* TLV serializer *)
+let parse_compositeDeviceID_sequence_TLV
+: parser _ compositeDeviceID_t_inbound
+= parse_asn1_sequence_TLV serialize_compositeDeviceID_value
+
+let serialize_compositeDeviceID_sequence_TLV
+: serializer parse_compositeDeviceID_sequence_TLV
+= serialize_asn1_sequence_TLV serialize_compositeDeviceID_value
+
+let serialize_compositeDeviceID_sequence_TLV_unfold
+= lemma_serialize_asn1_sequence_TLV_unfold serialize_compositeDeviceID_value
+
+let serialize_compositeDeviceID_sequence_TLV_size
+= lemma_serialize_asn1_sequence_TLV_size serialize_compositeDeviceID_value
+
+let serialize32_compositeDeviceID_value
+: serializer32_backwards serialize_compositeDeviceID_value
+= serialize32_synth_backwards
+  (* ls *) (serialize32_asn1_TLV_backwards_of_type INTEGER
+            `serialize32_nondep_then_backwards`
+            serialize32_subjectPublicKeyInfo_sequence_TLV_backwards
+            `serialize32_nondep_then_backwards`
+            serialize32_fwid_TLV_sequence_backwards)
+  (* f2 *) (synth_compositeDeviceID_t)
+  (* g1 *) (synth_compositeDeviceID_t')
+  (* g1'*) (synth_compositeDeviceID_t')
+  (* prf*) ()
+
+#push-options "--query_stats --z3rlimit 64"
+let len_of_compositeDeviceID_value_inbound
+  (x: compositeDeviceID_t_inbound)
+: Tot (inbound_sequence_value_len_of serialize_compositeDeviceID_value x)
+= serialize_compositeDeviceID_value_unfold x;
+  serialize_compositeDeviceID_value_size x;
+  len_of_asn1_primitive_TLV x.version +
+  len_of_subjectPublicKeyInfo_TLV_inbound x.deviceID +
+  len_of_fwid_TLV_inbound x.fwid2
+#pop-options
+
+let len_of_compositeDeviceID_TLV_inbound
+  (x: compositeDeviceID_t_inbound)
+// : Tot (inbound_sequence_value_len_of serialize_compositeDeviceID_sequence_TLV x)
+= len_of_sequence_TLV
+  (* s *) serialize_compositeDeviceID_value
+  (*len*) len_of_compositeDeviceID_value_inbound
+  (*val*) x
+
+let serialize32_compositeDeviceID_sequence
+: serializer32_backwards serialize_compositeDeviceID_sequence_TLV
+= serialize32_asn1_sequence_TLV_backwards
+  (* ls *) (serialize32_compositeDeviceID_value)
+  (*flen*) (len_of_compositeDeviceID_value_inbound)
