src/asn1/X509.Crypto.fst
@@ -1,0 +1,281 @@
+module X509.Crypto
+
+open LowParse.Low.Base
+// open LowParse.Low.Combinators
+
+open ASN1.Spec
+open ASN1.Low
+
+open X509.Base
+
+open FStar.Integers
+
+(* FIXME: ZT: large structs have bad performance. *)
+
+(* AlgorithmIdentifiers
+  ======================
+  NOTE: Different algorithms have identifiers in different structure.
+*)
+
+(* ECDSA Prime256 SHA2 *)
+noeq
+type algorithmIdentifier_ECDSA_P256_t = {
+  alg_id_oid_ecdsa: oid: datatype_of_asn1_type OID {oid == OID_EC_ALG_UNRESTRICTED};
+  alg_id_oid_p256 : oid: datatype_of_asn1_type OID {oid == OID_EC_GRP_SECP256R1}
+}
+
+/// tuple repr
+let filter_algorithmIdentifier_ECDSA_P256_t'
+  (x': tuple2 (datatype_of_asn1_type OID) (datatype_of_asn1_type OID))
+: GTot bool
+= fst x' = OID_EC_ALG_UNRESTRICTED &&
+  snd x' = OID_EC_GRP_SECP256R1
+
+let algorithmIdentifier_ECDSA_P256_t'
+= parse_filter_refine filter_algorithmIdentifier_ECDSA_P256_t'
+
+/// tuple repr -> record repr
+let synth_algorithmIdentifier_ECDSA_P256_t
+  (x': algorithmIdentifier_ECDSA_P256_t')
+: GTot (algorithmIdentifier_ECDSA_P256_t)
+= { alg_id_oid_ecdsa = fst x';
+    alg_id_oid_p256  = snd x' }
+
+/// record repr -> tuple repr
+let synth_algorithmIdentifier_ECDSA_P256_t'
+  (x: algorithmIdentifier_ECDSA_P256_t)
+: Tot (x': algorithmIdentifier_ECDSA_P256_t' { x == synth_algorithmIdentifier_ECDSA_P256_t x' })
+= (x.alg_id_oid_ecdsa, x.alg_id_oid_p256)
+
+/// sequence value (body) parser
+let parse_algorithmIdentifier_sequence_ECDSA_P256
+: parser _ algorithmIdentifier_ECDSA_P256_t
+= parse_asn1_TLV_of_type OID
+  `nondep_then`
+  parse_asn1_TLV_of_type OID
+  `parse_filter`
+  filter_algorithmIdentifier_ECDSA_P256_t'
+  `parse_synth`
+  synth_algorithmIdentifier_ECDSA_P256_t
+
+/// sequence value serializer
+let serialize_algorithmIdentifier_sequence_ECDSA_P256
+: serializer parse_algorithmIdentifier_sequence_ECDSA_P256
+= serialize_synth
+  (* p1 *) (parse_asn1_TLV_of_type OID
+            `nondep_then`
+            parse_asn1_TLV_of_type OID
+            `parse_filter`
+            filter_algorithmIdentifier_ECDSA_P256_t')
+  (* f2 *) (synth_algorithmIdentifier_ECDSA_P256_t)
+  (* s1 *) (serialize_asn1_TLV_of_type OID
+            `serialize_nondep_then`
+            serialize_asn1_TLV_of_type OID
+            `serialize_filter`
+            filter_algorithmIdentifier_ECDSA_P256_t')
+  (* g1 *) (synth_algorithmIdentifier_ECDSA_P256_t')
+  (* prf*) ()
+
+/// lemma: unfold sequence value serializer
+let lemma_serialize_algorithmIdentifier_sequence_ECDSA_P256_unfold
+  (x: algorithmIdentifier_ECDSA_P256_t)
+: Lemma (
+  serialize serialize_algorithmIdentifier_sequence_ECDSA_P256 x ==
+  serialize (serialize_asn1_TLV_of_type OID) x.alg_id_oid_ecdsa
+  `Seq.append`
+  serialize (serialize_asn1_TLV_of_type OID) x.alg_id_oid_p256
+)
+= serialize_nondep_then_eq
+  (* s1 *) (serialize_asn1_TLV_of_type OID)
+  (* s2 *) (serialize_asn1_TLV_of_type OID)
+  (* in *) (synth_algorithmIdentifier_ECDSA_P256_t' x);
+  serialize_synth_eq
+  (* p1 *) (parse_asn1_TLV_of_type OID
+            `nondep_then`
+            parse_asn1_TLV_of_type OID
+            `parse_filter`
+            filter_algorithmIdentifier_ECDSA_P256_t')
+  (* f2 *) (synth_algorithmIdentifier_ECDSA_P256_t)
+  (* s1 *) (serialize_asn1_TLV_of_type OID
+            `serialize_nondep_then`
+            serialize_asn1_TLV_of_type OID
+            `serialize_filter`
+            filter_algorithmIdentifier_ECDSA_P256_t')
+  (* g1 *) (synth_algorithmIdentifier_ECDSA_P256_t')
+  (* prf*) ()
+  (* in *) x
+
+/// lemma: reveal sequence serialization size
+let lemma_serialize_algorithmIdentifier_sequence_ECDSA_P256_size
+  (x: algorithmIdentifier_ECDSA_P256_t)
+: Lemma (
+  Seq.length (serialize serialize_algorithmIdentifier_sequence_ECDSA_P256 x) ==
+  length_of_asn1_primitive_TLV x.alg_id_oid_ecdsa +
+  length_of_asn1_primitive_TLV x.alg_id_oid_p256
+)
+= lemma_serialize_algorithmIdentifier_sequence_ECDSA_P256_unfold x
+
+/// inbound record repr
+let algorithmIdentifier_ECDSA_P256_t_inbound
+= inbound_sequence_value_of serialize_algorithmIdentifier_sequence_ECDSA_P256
+
+/// TLV
+///
+let parse_algorithmIdentifier_sequence_TLV_ECDSA_P256
+: parser _ algorithmIdentifier_ECDSA_P256_t_inbound
+= parse_asn1_sequence_TLV serialize_algorithmIdentifier_sequence_ECDSA_P256
+
+let serialize_algorithmIdentifier_sequence_TLV_ECDSA_P256
+: serializer parse_algorithmIdentifier_sequence_TLV_ECDSA_P256
+= serialize_asn1_sequence_TLV serialize_algorithmIdentifier_sequence_ECDSA_P256
+
+let lemma_serialize_algorithmIdentifier_sequence_TLV_ECDSA_P256_unfold
+= lemma_serialize_asn1_sequence_TLV_unfold serialize_algorithmIdentifier_sequence_ECDSA_P256
+
+let lemma_serialize_algorithmIdentifier_sequence_TLV_ECDSA_P256_size
+= lemma_serialize_asn1_sequence_TLV_size serialize_algorithmIdentifier_sequence_ECDSA_P256
+
+/// Low
+///
+
+inline_for_extraction
+let serialize32_algorithmIdentifier_sequence_ECDSA_P256_backwards
+: serializer32_backwards serialize_algorithmIdentifier_sequence_ECDSA_P256
+= serialize32_synth_backwards
+  (* ls *) (serialize32_asn1_TLV_backwards_of_type OID
+            `serialize32_nondep_then_backwards`
+            serialize32_asn1_TLV_backwards_of_type OID
+            `serialize32_filter_backwards`
+            filter_algorithmIdentifier_ECDSA_P256_t')
+  (* f2 *) (synth_algorithmIdentifier_ECDSA_P256_t)
+  (* g1 *) (synth_algorithmIdentifier_ECDSA_P256_t')
+  (* g1'*) (synth_algorithmIdentifier_ECDSA_P256_t')
+  (* prf*) ()
+
+let serialize32_algorithmIdentifier_sequence_TLV_ECDSA_P256_backwards
+: serializer32_backwards serialize_algorithmIdentifier_sequence_TLV_ECDSA_P256
+= serialize32_asn1_sequence_TLV_backwards
+  (* ls *) (serialize32_algorithmIdentifier_sequence_ECDSA_P256_backwards)
+
+
+(* SubjectPublicKeyInfo
+  ======================
+*)
+/// Record repr
+noeq
+type subjectPublicKeyInfo_ECDSA_P256_t = {
+  subjectPubKey_alg : algorithmIdentifier_ECDSA_P256_t_inbound;
+  subjectPubKey     : datatype_of_asn1_type BIT_STRING
+}
+
+/// tuple repr
+let subjectPublicKeyInfo_ECDSA_P256_t'
+= tuple2
+  (algorithmIdentifier_ECDSA_P256_t_inbound)
+  (datatype_of_asn1_type BIT_STRING)
+
+let synth_subjectPublicKeyInfo_ECDSA_P256_t
+  (x': subjectPublicKeyInfo_ECDSA_P256_t')
+: GTot (subjectPublicKeyInfo_ECDSA_P256_t)
+= { subjectPubKey_alg = fst x';
+    subjectPubKey     = snd x' }
+
+let synth_subjectPublicKeyInfo_ECDSA_P256_t'
+  (x: subjectPublicKeyInfo_ECDSA_P256_t)
+: Tot (x': subjectPublicKeyInfo_ECDSA_P256_t'{ x == synth_subjectPublicKeyInfo_ECDSA_P256_t x' })
+= (x.subjectPubKey_alg , x.subjectPubKey)
+
+let parse_subjectPublicKeyInfo_sequence_ECDSA_P256
+: parser _ (subjectPublicKeyInfo_ECDSA_P256_t)
+= parse_algorithmIdentifier_sequence_TLV_ECDSA_P256
+  `nondep_then`
+  parse_asn1_TLV_of_type BIT_STRING
+  `parse_synth`
+  synth_subjectPublicKeyInfo_ECDSA_P256_t
+
+let serialize_subjectPublicKeyInfo_sequence_ECDSA_P256
+: serializer (parse_subjectPublicKeyInfo_sequence_ECDSA_P256)
+= serialize_synth
+  (* p1 *) (parse_algorithmIdentifier_sequence_TLV_ECDSA_P256
+            `nondep_then`
+            parse_asn1_TLV_of_type BIT_STRING)
+  (* f2 *) (synth_subjectPublicKeyInfo_ECDSA_P256_t)
+  (* s1 *) (serialize_algorithmIdentifier_sequence_TLV_ECDSA_P256
+            `serialize_nondep_then`
+            serialize_asn1_TLV_of_type BIT_STRING)
+  (* g1 *) (synth_subjectPublicKeyInfo_ECDSA_P256_t')
+  (* prf*) ()
+
+let lemma_serialize_subjectPublicKeyInfo_sequence_ECDSA_P256_unfold
+  (x: subjectPublicKeyInfo_ECDSA_P256_t)
+: Lemma (
+  serialize (serialize_subjectPublicKeyInfo_sequence_ECDSA_P256) x ==
+  serialize (serialize_algorithmIdentifier_sequence_TLV_ECDSA_P256) x.subjectPubKey_alg
+  `Seq.append`
+  serialize (serialize_asn1_TLV_of_type BIT_STRING) x.subjectPubKey
+)
+= serialize_nondep_then_eq
+  (* s1 *) (serialize_algorithmIdentifier_sequence_TLV_ECDSA_P256)
+  (* s2 *) (serialize_asn1_TLV_of_type BIT_STRING)
+  (* in *) (synth_subjectPublicKeyInfo_ECDSA_P256_t' x);
+  serialize_synth_eq
+  (* p1 *) (parse_algorithmIdentifier_sequence_TLV_ECDSA_P256
+            `nondep_then`
+            parse_asn1_TLV_of_type BIT_STRING)
+  (* f2 *) (synth_subjectPublicKeyInfo_ECDSA_P256_t)
+  (* s1 *) (serialize_algorithmIdentifier_sequence_TLV_ECDSA_P256
+            `serialize_nondep_then`
+            serialize_asn1_TLV_of_type BIT_STRING)
+  (* g1 *) (synth_subjectPublicKeyInfo_ECDSA_P256_t')
+  (* prf*) ()
+  (* in *) x
+
+let lemma_serialize_subjectPublicKeyInfo_sequence_ECDSA_P256_size
+  (x: subjectPublicKeyInfo_ECDSA_P256_t)
+: Lemma (
+  Seq.length (serialize (serialize_subjectPublicKeyInfo_sequence_ECDSA_P256) x) ==
+  Seq.length (serialize (serialize_algorithmIdentifier_sequence_TLV_ECDSA_P256) x.subjectPubKey_alg) +
+  Seq.length (serialize (serialize_asn1_TLV_of_type BIT_STRING) x.subjectPubKey)
+)
+= lemma_serialize_subjectPublicKeyInfo_sequence_ECDSA_P256_unfold x
+
+(* NOTE: Define the `inbound` version of value type after we defined then serializer. *)
+let subjectPublicKeyInfo_ECDSA_P256_t_inbound
+= inbound_sequence_value_of (serialize_subjectPublicKeyInfo_sequence_ECDSA_P256)
+
+
+/// TLV
+///
+let parse_subjectPublicKeyInfo_sequence_TLV_ECDSA_P256
+: parser _ (subjectPublicKeyInfo_ECDSA_P256_t_inbound)
+= parse_asn1_sequence_TLV (serialize_subjectPublicKeyInfo_sequence_ECDSA_P256)
+
+let serialize_subjectPublicKeyInfo_sequence_TLV_ECDSA_P256
+: serializer (parse_subjectPublicKeyInfo_sequence_TLV_ECDSA_P256)
+= serialize_asn1_sequence_TLV (serialize_subjectPublicKeyInfo_sequence_ECDSA_P256)
+
+let lemma_serialize_subjectPublicKeyInfo_sequence_TLV_ECDSA_P256_unfold
+= lemma_serialize_asn1_sequence_TLV_unfold (serialize_subjectPublicKeyInfo_sequence_ECDSA_P256)
+
+let lemma_serialize_subjectPublicKeyInfo_sequence_TLV_ECDSA_P256_size
+= lemma_serialize_asn1_sequence_TLV_size (serialize_subjectPublicKeyInfo_sequence_ECDSA_P256)
+
+/// Low
+///
+
+inline_for_extraction
+let serialize32_subjectPublicKeyInfo_sequence_ECDSA_P256_backwards
+: serializer32_backwards (serialize_subjectPublicKeyInfo_sequence_ECDSA_P256)
+= serialize32_synth_backwards
+  (* ls *) (serialize32_algorithmIdentifier_sequence_TLV_ECDSA_P256_backwards
+            `serialize32_nondep_then_backwards`
+            serialize32_asn1_TLV_backwards_of_type BIT_STRING)
+  (* f2 *) (synth_subjectPublicKeyInfo_ECDSA_P256_t)
+  (* g1 *) (synth_subjectPublicKeyInfo_ECDSA_P256_t')
+  (* g1'*) (synth_subjectPublicKeyInfo_ECDSA_P256_t')
+  (* prf*) ()
+
+let serialize32_subjectPublicKeyInfo_sequence_TLV_ECDSA_P256_backwards
+: serializer32_backwards (serialize_subjectPublicKeyInfo_sequence_TLV_ECDSA_P256)
+= serialize32_asn1_sequence_TLV_backwards
+  (* ls *) (serialize32_subjectPublicKeyInfo_sequence_ECDSA_P256_backwards)
