src/asn1/X509.ExtFields.KeyUsage.fst
@@ -1,0 +1,205 @@
+module X509.ExtFields.KeyUsage
+
+open LowParse.Spec.Base
+open LowParse.Spec.Combinators
+
+open ASN1.Base
+open ASN1.Spec
+
+open X509.Base
+
+module B32 = FStar.Bytes
+
+open FStar.Integers
+
+(*
+/*
+ * X.509 v3 Key Usage Extension flags
+ * Reminder: update x509_info_key_usage() when adding new flags.
+ */
+#define MBEDTLS_X509_KU_DIGITAL_SIGNATURE            (0x80)  /* bit 0 */
+#define MBEDTLS_X509_KU_NON_REPUDIATION              (0x40)  /* bit 1 */
+#define MBEDTLS_X509_KU_KEY_ENCIPHERMENT             (0x20)  /* bit 2 */
+#define MBEDTLS_X509_KU_DATA_ENCIPHERMENT            (0x10)  /* bit 3 */
+#define MBEDTLS_X509_KU_KEY_AGREEMENT                (0x08)  /* bit 4 */
+#define MBEDTLS_X509_KU_KEY_CERT_SIGN                (0x04)  /* bit 5 */
+#define MBEDTLS_X509_KU_CRL_SIGN                     (0x02)  /* bit 6 */
+#define MBEDTLS_X509_KU_ENCIPHER_ONLY                (0x01)  /* bit 7 */
+#define MBEDTLS_X509_KU_DECIPHER_ONLY              (0x8000)  /* bit 8 */
+*)
+
+let key_usage_t = i: datatype_of_asn1_type INTEGER
+                     { 0l < i /\ (* at least one usage *)
+                      (i <= 0xFFl \/ i / 0x100l == 0x80l) }
+
+let x509_KU_DIGITAL_SIGNATURE :key_usage_t = 0x80l    (* bit 0 *)
+let x509_KU_NON_REPUDIATION   :key_usage_t = 0x40l    (* bit 1 *)
+let x509_KU_KEY_ENCIPHERMENT  :key_usage_t = 0x20l    (* bit 2 *)
+let x509_KU_DATA_ENCIPHERMENT :key_usage_t = 0x10l    (* bit 3 *)
+let x509_KU_KEY_AGREEMENT     :key_usage_t = 0x08l    (* bit 4 *)
+let x509_KU_KEY_CERT_SIGN     :key_usage_t = 0x04l    (* bit 5 *)
+let x509_KU_CRL_SIGN          :key_usage_t = 0x02l    (* bit 6 *)
+let x509_KU_ENCIPHER_ONLY     :key_usage_t = 0x01l    (* bit 7 *)
+let x509_KU_DECIPHER_ONLY     :key_usage_t = 0x8000l  (* bit 8 *)
+
+let filter_x509_key_usage
+  (bs: datatype_of_asn1_type BIT_STRING)
+: GTot bool
+= bs.bs_len = 3ul &&
+  bs.bs_unused_bits = 7ul &&
+  (* NOTE: RFC 5280 4.2.1.3:
+//            When the keyUsage extension appears in a certificate,
+//            at least one of the bits MUST be set to 1.*)
+  (B32.index bs.bs_s 1 = 0x80uy ||
+   B32.index bs.bs_s 1 = 0x00uy && B32.index bs.bs_s 0 > 0x00uy)
+
+let synth_x509_key_usage
+  (bs: parse_filter_refine filter_x509_key_usage)
+: GTot (key_usage_t)
+= cast #(Unsigned W8) #(Signed W32) (B32.index bs.bs_s 0) +
+  ((cast #(Unsigned W8) #(Signed W32) (B32.index bs.bs_s 1)) * 0x100l)
+
+let lemma_synth_x509_key_usage_injective'
+  (bs1 bs2: parse_filter_refine filter_x509_key_usage)
+: Lemma
+  (requires synth_x509_key_usage bs1 == synth_x509_key_usage bs2)
+  (ensures bs1 == bs2)
+= admit ()
+
+let lemma_synth_x509_key_usage_injective ()
+: Lemma (
+  synth_injective synth_x509_key_usage
+)
+= synth_injective_intro'
+  (* f *) synth_x509_key_usage
+  (*prf*) lemma_synth_x509_key_usage_injective'
+
+let synth_x509_key_usage_inverse
+  (ku: key_usage_t)
+: GTot (bs: parse_filter_refine filter_x509_key_usage
+            { synth_x509_key_usage bs == ku })
+= let b0: byte = cast (ku % 0x100l) in
+  let b1: byte = cast (ku / 0x100l) in
+  let s = Seq.createL [b0; b1] in
+  let s32 = B32.hide s in
+  { bs_len         = 3ul;
+    bs_unused_bits = 7ul;
+    bs_s           = s32 }
+
+let parse_x509_key_usage
+: parser _ key_usage_t
+= lemma_synth_x509_key_usage_injective ();
+  parse_asn1_TLV_of_type BIT_STRING
+  `parse_filter`
+  filter_x509_key_usage
+  `parse_synth`
+  synth_x509_key_usage
+
+let serialize_x509_key_usage
+: serializer parse_x509_key_usage
+= serialize_synth
+  (* p1 *) (parse_asn1_TLV_of_type BIT_STRING
+            `parse_filter`
+            filter_x509_key_usage)
+  (* f2 *) (synth_x509_key_usage)
+  (* s1 *) (serialize_asn1_TLV_of_type BIT_STRING
+            `serialize_filter`
+            filter_x509_key_usage)
+  (* g1 *) (synth_x509_key_usage_inverse)
+  (* Prf*) (lemma_synth_x509_key_usage_injective ())
+
+let lemma_serialize_x509_key_usage_unfold
+  (ku: key_usage_t)
+: Lemma (
+  serialize serialize_x509_key_usage ku ==
+  serialize (serialize_asn1_TLV_of_type BIT_STRING) (synth_x509_key_usage_inverse ku)
+)
+= serialize_synth_eq
+  (* p1 *) (parse_asn1_TLV_of_type BIT_STRING
+            `parse_filter`
+            filter_x509_key_usage)
+  (* f2 *) (synth_x509_key_usage)
+  (* s1 *) (serialize_asn1_TLV_of_type BIT_STRING
+            `serialize_filter`
+            filter_x509_key_usage)
+  (* g1 *) (synth_x509_key_usage_inverse)
+  (* Prf*) (lemma_synth_x509_key_usage_injective ())
+  (* in *) (ku)
+
+let lemma_serialize_x509_key_usage_size
+  (ku: key_usage_t)
+: Lemma (
+  Seq.length (serialize serialize_x509_key_usage ku) ==
+  length_of_asn1_primitive_TLV #BIT_STRING (synth_x509_key_usage_inverse ku)
+)
+= lemma_serialize_x509_key_usage_unfold ku
+
+// let parse_envelop_OID_with
+//   (oid: datatype_of_asn1_type OID)
+//   (#k: parser_kind)
+//   (#t: Type0)
+//   (#p: parser k t)
+//   (s: serializer p)
+// : parser _ _
+// = parse_asn1_oid_TLV
+//   `parse_filter`
+//   (fun x -> x = oid)
+//   `nondep_then`
+//   p
+
+let parse_x509_key_usage_sequence_TLV
+= parse_asn1_sequence_TLV
+    (OID_KEY_USAGE
+     `serialize_envelop_OID_with`
+     serialize_x509_key_usage)
+
+let serialize_x509_key_usage_sequence_TLV
+= serialize_asn1_sequence_TLV
+    (OID_KEY_USAGE
+     `serialize_envelop_OID_with`
+     serialize_x509_key_usage)
+
+let lemma_serialize_x509_key_usage_sequence_TLV_unfold
+= lemma_serialize_asn1_sequence_TLV_unfold
+    (OID_KEY_USAGE
+     `serialize_envelop_OID_with`
+     serialize_x509_key_usage)
+
+let lemma_serialize_x509_key_usage_sequence_TLV_size
+= lemma_serialize_asn1_sequence_TLV_size
+    (OID_KEY_USAGE
+     `serialize_envelop_OID_with`
+     serialize_x509_key_usage)
+
+open ASN1.Low
+
+let synth_x509_key_usage_inverse_impl
+  (ku: key_usage_t)
+: Tot (bs: parse_filter_refine filter_x509_key_usage
+           { bs == synth_x509_key_usage_inverse ku })
+= let b0: byte = cast (ku % 0x100l) in
+  let b1: byte = cast (ku / 0x100l) in
+  let s32 = B32.(create 1ul b0 `append` create 1ul b1) in
+  (* Prf *) B32.extensionality s32 (B32.hide (Seq.createL [b0; b1]));
+  { bs_len         = 3ul;
+    bs_unused_bits = 7ul;
+    bs_s           = s32 }
+
+let serialize32_x509_key_usage_backwards
+: serializer32_backwards (serialize_x509_key_usage)
+= serialize32_synth_backwards
+  (* s1 *) (serialize32_asn1_TLV_backwards_of_type BIT_STRING
+            `serialize32_filter_backwards`
+            filter_x509_key_usage)
+  (* f2 *) (synth_x509_key_usage)
+  (* g1 *) (synth_x509_key_usage_inverse)
+  (* g1'*) (synth_x509_key_usage_inverse_impl)
+  (* prf*) (lemma_synth_x509_key_usage_injective ())
+
+let serialize32_x509_key_usage_sequence_TLV_backwards
+: serializer32_backwards (serialize_x509_key_usage_sequence_TLV)
+= lemma_synth_x509_key_usage_injective ();
+  serialize32_asn1_sequence_TLV_backwards
+    (OID_KEY_USAGE
+     `serialize32_envelop_OID_with_backwards`
+     serialize32_x509_key_usage_backwards)
