src/asn1/X509.Extension.fst
@@ -1,0 +1,242 @@
+module X509.Extension
+
+open LowParse.Spec.Base
+open LowParse.Spec.Combinators
+
+open ASN1.Base
+open ASN1.Spec
+
+open X509.Base
+
+module B32 = FStar.Bytes
+
+noeq
+type x509_extension_t
+  (#k: parser_kind)
+  (#t: Type0)
+  (#p: parser k t)
+  (s: serializer p)
+= { x509_extID      : datatype_of_asn1_type OID;
+    x509_extCritical: datatype_of_asn1_type BOOLEAN;
+    x509_extValue   : OCTET_STRING `inbound_envelop_tag_with_value_of` s }
+
+/// tuple repr
+let x509_extension_t'
+  (#k: parser_kind)
+  (#t: Type0)
+  (#p: parser k t)
+  (s: serializer p)
+= datatype_of_asn1_type OID
+  `tuple2`
+  datatype_of_asn1_type BOOLEAN
+  `tuple2`
+ (OCTET_STRING `inbound_envelop_tag_with_value_of` s)
+
+let synth_x509_extension_t
+  (#k: parser_kind)
+  (#t: Type0)
+  (#p: parser k t)
+  (s: serializer p)
+  (x': x509_extension_t' s)
+: GTot (x509_extension_t s)
+= { x509_extID       = fst (fst x');
+    x509_extCritical = snd (fst x');
+    x509_extValue    = snd x' }
+
+let synth_x509_extension_t'
+  (#k: parser_kind)
+  (#t: Type0)
+  (#p: parser k t)
+  (s: serializer p)
+  (x: x509_extension_t s)
+: GTot (x': x509_extension_t' s { x == synth_x509_extension_t s x' })
+= (x.x509_extID, x.x509_extCritical), x.x509_extValue
+
+let parse_x509_extension
+  (#k: parser_kind)
+  (#t: Type0)
+  (#p: parser k t)
+  (s: serializer p)
+: parser _ (x509_extension_t s)
+= parse_asn1_TLV_of_type OID
+  `nondep_then`
+  parse_asn1_TLV_of_type BOOLEAN
+  `nondep_then`
+ (OCTET_STRING
+  `parse_asn1_envelop_tag_with_TLV`
+  s)
+  `parse_synth`
+  synth_x509_extension_t s
+
+let serialize_x509_extension
+  (#k: parser_kind)
+  (#t: Type0)
+  (#p: parser k t)
+  (s: serializer p)
+: serializer (parse_x509_extension s)
+= serialize_synth
+  (* p1 *) (parse_asn1_TLV_of_type OID
+            `nondep_then`
+            parse_asn1_TLV_of_type BOOLEAN
+            `nondep_then`
+           (OCTET_STRING
+            `parse_asn1_envelop_tag_with_TLV`
+            s))
+  (* f2 *) (synth_x509_extension_t s)
+  (* s1 *) (serialize_asn1_TLV_of_type OID
+            `serialize_nondep_then`
+            serialize_asn1_TLV_of_type BOOLEAN
+            `serialize_nondep_then`
+           (OCTET_STRING
+            `serialize_asn1_envelop_tag_with_TLV`
+            s))
+  (* g1 *) (synth_x509_extension_t' s)
+  (* prf*) ()
+
+let lemma_serialize_x509_extension_unfold
+  (#k: parser_kind)
+  (#t: Type0)
+  (#p: parser k t)
+  (s: serializer p)
+  (x: x509_extension_t s)
+: Lemma (
+  serialize (serialize_x509_extension s) x ==
+  serialize (serialize_asn1_TLV_of_type OID) x.x509_extID
+  `Seq.append`
+  serialize (serialize_asn1_TLV_of_type BOOLEAN) x.x509_extCritical
+  `Seq.append`
+  serialize (OCTET_STRING `serialize_asn1_envelop_tag_with_TLV` s) x.x509_extValue
+)
+= serialize_nondep_then_eq
+  (* s1 *) (serialize_asn1_TLV_of_type OID)
+  (* s2 *) (serialize_asn1_TLV_of_type BOOLEAN)
+  (* in *) (fst (synth_x509_extension_t' s x));
+  serialize_nondep_then_eq
+  (* s1 *) (serialize_asn1_TLV_of_type OID
+            `serialize_nondep_then`
+            serialize_asn1_TLV_of_type BOOLEAN)
+  (* s2 *) (OCTET_STRING
+            `serialize_asn1_envelop_tag_with_TLV`
+            s)
+  (* in *) (synth_x509_extension_t' s x);
+  serialize_synth_eq
+  (* p1 *) (parse_asn1_TLV_of_type OID
+            `nondep_then`
+            parse_asn1_TLV_of_type BOOLEAN
+            `nondep_then`
+           (OCTET_STRING
+            `parse_asn1_envelop_tag_with_TLV`
+            s))
+  (* f2 *) (synth_x509_extension_t s)
+  (* s1 *) (serialize_asn1_TLV_of_type OID
+            `serialize_nondep_then`
+            serialize_asn1_TLV_of_type BOOLEAN
+            `serialize_nondep_then`
+           (OCTET_STRING
+            `serialize_asn1_envelop_tag_with_TLV`
+            s))
+  (* g1 *) (synth_x509_extension_t' s)
+  (* prf*) ()
+  (* in *) x
+
+let lemma_serialize_x509_extension_size
+  (#k: parser_kind)
+  (#t: Type0)
+  (#p: parser k t)
+  (s: serializer p)
+  (x: x509_extension_t s)
+: Lemma (
+  Seq.length (serialize (serialize_x509_extension s) x) ==
+  length_of_asn1_primitive_TLV x.x509_extID +
+  length_of_asn1_primitive_TLV x.x509_extCritical +
+  Seq.length (serialize (OCTET_STRING `serialize_asn1_envelop_tag_with_TLV` s) x.x509_extValue)
+)
+= lemma_serialize_x509_extension_unfold s x
+
+unfold
+let x509_extension_t_inbound
+  (#k: parser_kind)
+  (#t: Type0)
+  (#p: parser k t)
+  (s: serializer p)
+= inbound_sequence_value_of s
+
+/// SEQUENCE TLV
+
+unfold
+let parse_x509_extension_sequence_TLV
+  (#k: parser_kind)
+  (#t: Type0)
+  (#p: parser k t)
+  (s: serializer p)
+= parse_asn1_sequence_TLV
+  (* s *) (serialize_x509_extension s)
+
+unfold
+let serialize_x509_extension_sequence_TLV
+  (#k: parser_kind)
+  (#t: Type0)
+  (#p: parser k t)
+  (s: serializer p)
+: serializer (parse_x509_extension_sequence_TLV s)
+= serialize_asn1_sequence_TLV
+  (* s *) (serialize_x509_extension s)
+
+unfold
+let lemma_serialize_x509_extension_sequence_TLV_unfold
+  (#k: parser_kind)
+  (#t: Type0)
+  (#p: parser k t)
+  (s: serializer p)
+= lemma_serialize_asn1_sequence_TLV_unfold
+  (* s *) (serialize_x509_extension s)
+
+unfold
+let lemma_serialize_x509_extension_sequence_TLV_size
+  (#k: parser_kind)
+  (#t: Type0)
+  (#p: parser k t)
+  (s: serializer p)
+= lemma_serialize_asn1_sequence_TLV_size
+  (* s *) (serialize_x509_extension s)
+
+open ASN1.Low
+
+let synth_x509_extension_t'_impl
+  (#k: parser_kind)
+  (#t: Type0)
+  (#p: parser k t)
+  (s: serializer p)
+  (x: x509_extension_t s)
+: Tot (x': x509_extension_t' s { x' == synth_x509_extension_t' s x })
+= (x.x509_extID, x.x509_extCritical), x.x509_extValue
+
+let serialize32_x509_extension_backwards
+  (#k: parser_kind)
+  (#t: Type0)
+  (#p: parser k t)
+  (#s: serializer p)
+  (s32: serializer32_backwards s)
+: serializer32_backwards (serialize_x509_extension s)
+= serialize32_synth_backwards
+  (* s32*) (serialize32_asn1_TLV_backwards_of_type OID
+            `serialize32_nondep_then_backwards`
+            serialize32_asn1_TLV_backwards_of_type BOOLEAN
+            `serialize32_nondep_then_backwards`
+           (OCTET_STRING
+            `serialize32_asn1_envelop_tag_with_TLV_backwards`
+            s32))
+  (* f2 *) (synth_x509_extension_t s)
+  (* g1 *) (synth_x509_extension_t' s)
+  (* g1'*) (synth_x509_extension_t'_impl s)
+  (* prf*) ()
+
+let serialize32_x509_extension_sequence_TLV_backwards
+  (#k: parser_kind)
+  (#t: Type0)
+  (#p: parser k t)
+  (#s: serializer p)
+  (s32: serializer32_backwards s)
+: serializer32_backwards (serialize_x509_extension_sequence_TLV s)
+= serialize32_asn1_sequence_TLV_backwards
+  (* s32 *) (serialize32_x509_extension_backwards s32)
