src/asn1/X509.RIoT.Ext.fst
@@ -1,0 +1,392 @@
+module X509.RIoT.Ext
+
+open LowParse.Low.Base
+// open LowParse.Low.Combinators
+
+open ASN1.Spec
+open ASN1.Low
+
+open X509.Crypto
+
+(* FWID
+  ======
+*)
+noeq
+type fwid_t = {
+  fwid_hashAlg: datatype_of_asn1_type OID; (* OID *)
+  fwid_value  : datatype_of_asn1_type OCTET_STRING
+}
+let fwid_t' = (datatype_of_asn1_type OID & datatype_of_asn1_type OCTET_STRING)
+
+(* Serialier spec *)
+let synth_fwid_t
+  (x': fwid_t')
+: GTot (fwid_t)
+= { fwid_hashAlg = fst x';
+    fwid_value   = snd x' }
+
+let synth_fwid_t'
+  (x: fwid_t)
+: Tot (x': fwid_t' { x == synth_fwid_t x' } )
+= (x.fwid_hashAlg, x.fwid_value)
+
+let parse_fwid_sequence
+: parser _ fwid_t
+= parse_asn1_TLV_of_type OID
+  `nondep_then`
+  parse_asn1_TLV_of_type OCTET_STRING
+  `parse_synth`
+  synth_fwid_t
+
+let serialize_fwid_sequence
+: serializer parse_fwid_sequence
+= serialize_synth
+  (* p1 *) (parse_asn1_TLV_of_type OID
+            `nondep_then`
+            parse_asn1_TLV_of_type OCTET_STRING)
+  (* f2 *) (synth_fwid_t)
+  (* s1 *) (serialize_asn1_TLV_of_type OID
+            `serialize_nondep_then`
+            serialize_asn1_TLV_of_type OCTET_STRING)
+  (* g1 *) (synth_fwid_t')
+  (* prf*) ()
+
+let lemma_serialize_fwid_sequence_unfold
+  (x: fwid_t)
+: Lemma (
+  serialize serialize_fwid_sequence x ==
+  serialize serialize_asn1_oid_TLV x.fwid_hashAlg
+  `Seq.append`
+  serialize serialize_asn1_octet_string_TLV x.fwid_value
+)
+= serialize_nondep_then_eq
+  (* s1 *) (serialize_asn1_TLV_of_type OID)
+  (* s2 *) (serialize_asn1_TLV_of_type OCTET_STRING)
+  (* in *) (synth_fwid_t' x);
+  serialize_synth_eq
+  (* p1 *) (parse_asn1_TLV_of_type OID
+            `nondep_then`
+            parse_asn1_TLV_of_type OCTET_STRING)
+  (* f2 *) (synth_fwid_t)
+  (* s1 *) (serialize_asn1_TLV_of_type OID
+            `serialize_nondep_then`
+            serialize_asn1_TLV_of_type OCTET_STRING)
+  (* g1 *) (synth_fwid_t')
+  (* prf*) ()
+  (* in *) x
+
+#push-options "--query_stats --z3rlimit 16"
+let lemma_serialize_fwid_sequence_size
+  (x: fwid_t)
+: Lemma (
+  Seq.length (serialize serialize_fwid_sequence x) ==
+  length_of_asn1_primitive_TLV x.fwid_hashAlg +
+  length_of_asn1_primitive_TLV x.fwid_value
+)
+= lemma_serialize_fwid_sequence_unfold x;
+  lemma_serialize_asn1_oid_TLV_size x.fwid_hashAlg;
+  lemma_serialize_asn1_octet_string_TLV_size x.fwid_value
+#pop-options
+
+(* inbound sub type*)
+let fwid_t_inbound
+= inbound_sequence_value_of serialize_fwid_sequence
+
+(* TLV serializer *)
+let parse_fwid_sequence_TLV
+: parser _ fwid_t_inbound
+= parse_asn1_sequence_TLV serialize_fwid_sequence
+
+let serialize_fwid_sequence_TLV
+: serializer parse_fwid_sequence_TLV
+= serialize_asn1_sequence_TLV serialize_fwid_sequence
+
+let lemma_serialize_fwid_sequence_TLV_unfold
+= lemma_serialize_asn1_sequence_TLV_unfold serialize_fwid_sequence
+
+let lemma_serialize_fwid_sequence_TLV_size
+= lemma_serialize_asn1_sequence_TLV_size serialize_fwid_sequence
+
+let serialize32_fwid_sequence
+: serializer32_backwards serialize_fwid_sequence
+= serialize32_synth_backwards
+  (* ls *) (serialize32_asn1_TLV_backwards_of_type OID
+            `serialize32_nondep_then_backwards`
+            serialize32_asn1_TLV_backwards_of_type OCTET_STRING)
+  (* f2 *) (synth_fwid_t)
+  (* g1 *) (synth_fwid_t')
+  (* g1'*) (synth_fwid_t')
+  (* prf*) ()
+
+let serialize32_fwid_TLV_sequence_backwards
+: serializer32_backwards serialize_fwid_sequence_TLV
+= serialize32_asn1_sequence_TLV_backwards
+  (* ls *) (serialize32_fwid_sequence)
+
+(* CompositeDeviceID *)
+noeq
+type compositeDeviceID_t = {
+  device_version: datatype_of_asn1_type INTEGER;
+  deviceID: subjectPublicKeyInfo_ECDSA_P256_t_inbound;
+  fwid: fwid_t_inbound
+}
+
+let compositeDeviceID_t'
+= ((datatype_of_asn1_type INTEGER &
+    subjectPublicKeyInfo_ECDSA_P256_t_inbound) &
+    fwid_t_inbound)
+
+(* Serialier spec *)
+let synth_compositeDeviceID_t
+  (x': compositeDeviceID_t')
+: GTot (compositeDeviceID_t)
+= { device_version  = fst (fst x');
+    deviceID = snd (fst x');
+    fwid     = snd x' }
+
+let synth_compositeDeviceID_t'
+  (x: compositeDeviceID_t)
+: Tot (x': compositeDeviceID_t' { x == synth_compositeDeviceID_t x' })
+= ((x.device_version, x.deviceID), x.fwid)
+
+let parse_compositeDeviceID_sequence
+: parser _ compositeDeviceID_t
+= parse_asn1_TLV_of_type INTEGER
+  `nondep_then`
+  parse_subjectPublicKeyInfo_sequence_TLV_ECDSA_P256
+  `nondep_then`
+  parse_fwid_sequence_TLV
+  `parse_synth`
+  synth_compositeDeviceID_t
+
+let serialize_compositeDeviceID_sequence
+: serializer parse_compositeDeviceID_sequence
+= serialize_synth
+  (* p1 *) (parse_asn1_TLV_of_type INTEGER
+            `nondep_then`
+            parse_subjectPublicKeyInfo_sequence_TLV_ECDSA_P256
+            `nondep_then`
+            parse_fwid_sequence_TLV)
+  (* f2 *) (synth_compositeDeviceID_t)
+  (* s1 *) (serialize_asn1_TLV_of_type INTEGER
+            `serialize_nondep_then`
+            serialize_subjectPublicKeyInfo_sequence_TLV_ECDSA_P256
+            `serialize_nondep_then`
+            serialize_fwid_sequence_TLV)
+  (* g1 *) (synth_compositeDeviceID_t')
+  (* prf*) ()
+
+let lemma_serialize_compositeDeviceID_sequence_unfold
+  (x: compositeDeviceID_t)
+: Lemma (
+  serialize serialize_compositeDeviceID_sequence x ==
+  serialize (serialize_asn1_TLV_of_type INTEGER) x.device_version
+  `Seq.append`
+  serialize serialize_subjectPublicKeyInfo_sequence_TLV_ECDSA_P256 x.deviceID
+  `Seq.append`
+  serialize serialize_fwid_sequence_TLV x.fwid
+)
+= serialize_nondep_then_eq
+  (* s1 *) (serialize_asn1_TLV_of_type INTEGER)
+  (* s2 *) (serialize_subjectPublicKeyInfo_sequence_TLV_ECDSA_P256)
+  (* in *) (fst (synth_compositeDeviceID_t' x));
+  serialize_nondep_then_eq
+  (* s1 *) (serialize_asn1_TLV_of_type INTEGER
+            `serialize_nondep_then`
+            serialize_subjectPublicKeyInfo_sequence_TLV_ECDSA_P256)
+  (* s2 *) (serialize_fwid_sequence_TLV)
+  (* in *) (synth_compositeDeviceID_t' x);
+  serialize_synth_eq
+  (* p1 *) (parse_asn1_TLV_of_type INTEGER
+            `nondep_then`
+            parse_subjectPublicKeyInfo_sequence_TLV_ECDSA_P256
+            `nondep_then`
+            parse_fwid_sequence_TLV)
+  (* f2 *) (synth_compositeDeviceID_t)
+  (* s1 *) (serialize_asn1_TLV_of_type INTEGER
+            `serialize_nondep_then`
+            serialize_subjectPublicKeyInfo_sequence_TLV_ECDSA_P256
+            `serialize_nondep_then`
+            serialize_fwid_sequence_TLV)
+  (* g1 *) (synth_compositeDeviceID_t')
+  (* prf*) ()
+  (* in *) x
+
+let lemma_serialize_compositeDeviceID_sequence_size
+  (x: compositeDeviceID_t)
+: Lemma (
+  Seq.length (serialize serialize_compositeDeviceID_sequence x) ==
+  length_of_asn1_primitive_TLV x.device_version +
+  Seq.length (serialize serialize_subjectPublicKeyInfo_sequence_TLV_ECDSA_P256 x.deviceID) +
+  Seq.length (serialize serialize_fwid_sequence_TLV x.fwid))
+= lemma_serialize_compositeDeviceID_sequence_unfold x;
+  lemma_serialize_asn1_integer_TLV_size x.device_version;
+  lemma_serialize_subjectPublicKeyInfo_sequence_TLV_ECDSA_P256_size x.deviceID;
+  lemma_serialize_fwid_sequence_TLV_size x.fwid
+
+(* inbound sub type*)
+let compositeDeviceID_t_inbound
+= inbound_sequence_value_of serialize_compositeDeviceID_sequence
+
+(* TLV serializer *)
+let parse_compositeDeviceID_sequence_TLV
+: parser _ compositeDeviceID_t_inbound
+= parse_asn1_sequence_TLV serialize_compositeDeviceID_sequence
+
+let serialize_compositeDeviceID_sequence_TLV
+: serializer parse_compositeDeviceID_sequence_TLV
+= serialize_asn1_sequence_TLV serialize_compositeDeviceID_sequence
+
+let lemma_serialize_compositeDeviceID_sequence_TLV_unfold
+= lemma_serialize_asn1_sequence_TLV_unfold serialize_compositeDeviceID_sequence
+
+let lemma_serialize_compositeDeviceID_sequence_TLV_size
+= lemma_serialize_asn1_sequence_TLV_size serialize_compositeDeviceID_sequence
+
+let serialize32_compositeDeviceID_sequence
+: serializer32_backwards serialize_compositeDeviceID_sequence
+= serialize32_synth_backwards
+  (* ls *) (serialize32_asn1_TLV_backwards_of_type INTEGER
+            `serialize32_nondep_then_backwards`
+            serialize32_subjectPublicKeyInfo_sequence_TLV_ECDSA_P256_backwards
+            `serialize32_nondep_then_backwards`
+            serialize32_fwid_TLV_sequence_backwards)
+  (* f2 *) (synth_compositeDeviceID_t)
+  (* g1 *) (synth_compositeDeviceID_t')
+  (* g1'*) (synth_compositeDeviceID_t')
+  (* prf*) ()
+
+let serialize32_compositeDeviceID_TLV_sequence_backwards
+: serializer32_backwards serialize_compositeDeviceID_sequence_TLV
+= serialize32_asn1_sequence_TLV_backwards
+  (* ls *) (serialize32_compositeDeviceID_sequence)
+
+(* RIoT Extension*)
+noeq
+type riot_extension_t = {
+  riot_oid: oid:datatype_of_asn1_type OID{ oid == OID_RIOT };
+  riot_compositeDeviceID: compositeDeviceID_t_inbound
+}
+
+/// tuple repr
+let filter_riot_extension_t'
+  (x': tuple2 (datatype_of_asn1_type OID) compositeDeviceID_t_inbound)
+: GTot bool
+= fst x' = OID_RIOT
+
+let riot_extension_t'
+= parse_filter_refine filter_riot_extension_t'
+
+(* Serialier spec *)
+let synth_riot_extension_t
+  (x': riot_extension_t')
+: GTot (riot_extension_t)
+= { riot_oid = fst x';
+    riot_compositeDeviceID = snd x' }
+
+let synth_riot_extension_t'
+  (x: riot_extension_t)
+: Tot (x': riot_extension_t' { x == synth_riot_extension_t x' })
+= (x.riot_oid, x.riot_compositeDeviceID)
+
+let parse_riot_extension_sequence
+: parser _ riot_extension_t
+= parse_asn1_TLV_of_type OID
+  `nondep_then`
+  parse_compositeDeviceID_sequence_TLV
+  `parse_filter`
+  filter_riot_extension_t'
+  `parse_synth`
+  synth_riot_extension_t
+
+let serialize_riot_extension_sequence
+: serializer parse_riot_extension_sequence
+= serialize_synth
+  (* p1 *) (parse_asn1_TLV_of_type OID
+            `nondep_then`
+            parse_compositeDeviceID_sequence_TLV
+            `parse_filter`
+            filter_riot_extension_t')
+  (* f2 *) (synth_riot_extension_t)
+  (* s1 *) (serialize_asn1_TLV_of_type OID
+            `serialize_nondep_then`
+            serialize_compositeDeviceID_sequence_TLV
+            `serialize_filter`
+            filter_riot_extension_t')
+  (* g1 *) (synth_riot_extension_t')
+  (* prf*) ()
+
+let lemma_serialize_riot_extension_sequence_unfold
+  (x: riot_extension_t)
+: Lemma (
+  serialize serialize_riot_extension_sequence x ==
+  serialize (serialize_asn1_TLV_of_type OID) x.riot_oid
+  `Seq.append`
+  serialize serialize_compositeDeviceID_sequence_TLV x.riot_compositeDeviceID
+)
+= serialize_nondep_then_eq
+  (* s1 *) (serialize_asn1_TLV_of_type OID)
+  (* s2 *) (serialize_compositeDeviceID_sequence_TLV)
+  (* in *) (synth_riot_extension_t' x);
+  serialize_synth_eq
+  (* p1 *) (parse_asn1_TLV_of_type OID
+            `nondep_then`
+            parse_compositeDeviceID_sequence_TLV
+            `parse_filter`
+            filter_riot_extension_t')
+  (* f2 *) (synth_riot_extension_t)
+  (* s1 *) (serialize_asn1_TLV_of_type OID
+            `serialize_nondep_then`
+            serialize_compositeDeviceID_sequence_TLV
+            `serialize_filter`
+            filter_riot_extension_t')
+  (* g1 *) (synth_riot_extension_t')
+  (* prf*) ()
+  (* in *) x
+
+let lemma_serialize_riot_extension_sequence_size
+  (x: riot_extension_t)
+: Lemma (
+  Seq.length (serialize serialize_riot_extension_sequence x) ==
+  length_of_asn1_primitive_TLV x.riot_oid +
+  Seq.length (serialize serialize_compositeDeviceID_sequence_TLV x.riot_compositeDeviceID))
+= lemma_serialize_riot_extension_sequence_unfold x;
+  lemma_serialize_asn1_oid_TLV_size x.riot_oid;
+  lemma_serialize_compositeDeviceID_sequence_TLV_size x.riot_compositeDeviceID
+
+(* inbound sub type*)
+let riot_extension_t_inbound
+= inbound_sequence_value_of serialize_riot_extension_sequence
+
+(* TLV serializer *)
+let parse_riot_extension_sequence_TLV
+: parser _ riot_extension_t_inbound
+= parse_asn1_sequence_TLV serialize_riot_extension_sequence
+
+let serialize_riot_extension_sequence_TLV
+: serializer parse_riot_extension_sequence_TLV
+= serialize_asn1_sequence_TLV serialize_riot_extension_sequence
+
+let lemma_serialize_riot_extension_sequence_TLV_unfold
+= lemma_serialize_asn1_sequence_TLV_unfold serialize_riot_extension_sequence
+
+let lemma_serialize_riot_extension_sequence_TLV_size
+= lemma_serialize_asn1_sequence_TLV_size serialize_riot_extension_sequence
+
+let serialize32_riot_extension_sequence
+: serializer32_backwards serialize_riot_extension_sequence
+= serialize32_synth_backwards
+  (* ls *) (serialize32_asn1_TLV_backwards_of_type OID
+            `serialize32_nondep_then_backwards`
+            serialize32_compositeDeviceID_TLV_sequence_backwards
+            `serialize32_filter_backwards`
+            filter_riot_extension_t')
+  (* f2 *) (synth_riot_extension_t)
+  (* g1 *) (synth_riot_extension_t')
+  (* g1'*) (synth_riot_extension_t')
+  (* prf*) ()
+
+let serialize32_riot_extension_TLV_sequence_backwards
+: serializer32_backwards serialize_riot_extension_sequence_TLV
+= serialize32_asn1_sequence_TLV_backwards
+  (* ls *) (serialize32_riot_extension_sequence)
